theories/rules.v
@@ -47,7 +47,6 @@ Section cap_lang_rules.
   Implicit Types P Q : iProp Σ.
   Implicit Types σ : ExecConf.
   Implicit Types c : cap_lang.expr. 
-  Implicit Types e : option Addr.
   Implicit Types a b : Addr.
   Implicit Types r : RegName.
   Implicit Types v : cap_lang.val. 
@@ -257,7 +256,7 @@ Section cap_lang_rules.
        Instr Executable @ E
        {{{ RET NextIV;
            PC ↦ᵣ inr ((pc_p,pc_g),pc_b,pc_e,pc_a')
-           ∗ dst ↦ᵣ inr (p, g, a1, if (a2 =? -42)%a then None else Some a2, a)
+           ∗ dst ↦ᵣ inr (p, g, a1, if (a2 =? -42)%a then A MemNum eq_refl else a2, a)
        }}}.
    Proof.
      iIntros (Hinstr Hvpc Hpca' [Hn1 Hn2] Hpne Hdstne Hwb ϕ) "(>HPC & >Hpc_a & >Hdst & >Hr1 & >Hr2) Hϕ".
@@ -270,8 +269,8 @@ Section cap_lang_rules.
      iDestruct (@gen_heap_valid with "Hr Hr1") as %?.
      iDestruct (@gen_heap_valid with "Hr Hr2") as %?.
      option_locate_mr m r.
-     assert (<[dst:=inr (p, g, a1, if (a2 =? -42)%a then None
-                                   else Some a2, a)]>
+     assert (<[dst:=inr (p, g, a1, if (a2 =? -42)%a then (A MemNum eq_refl)
+                                   else a2, a)]>
              r !r! PC = (inr (pc_p, pc_g, pc_b, pc_e, pc_a)))
        as Hpc_new1.
      { rewrite (locate_ne_reg _ _ _ (inr (pc_p, pc_g, pc_b, pc_e, pc_a))); eauto. }
@@ -280,7 +279,7 @@ Section cap_lang_rules.
      - rewrite /reducible.
        iExists [], (Instr _),
        (updatePC (update_reg (r,m) dst (inr ((p, g), a1,
-            if (a2 =? (-42))%a then None else Some a2, a)))).2,[].
+            if (a2 =? (-42))%a then (A MemNum eq_refl) else a2, a)))).2,[].
        iPureIntro.
        constructor.
        apply (step_exec_instr (r,m) pc_p pc_g pc_b pc_e pc_a
@@ -316,7 +315,7 @@ Section cap_lang_rules.
            ∗ ▷ r2 ↦ᵣ inl n2 }}}
        Instr Executable @ E
        {{{ RET NextIV;
-           PC ↦ᵣ inr ((pc_p,pc_g),a1,if (a2 =? -42)%a then None else Some a2,pc_a')
+           PC ↦ᵣ inr ((pc_p,pc_g),a1,if (a2 =? -42)%a then (A MemNum eq_refl) else a2,pc_a')
         }}}.
    Proof.
      iIntros (Hinstr Hvpc Hpca' [Hn1 Hn2] Hpne Hwb ϕ) "(>HPC & >Hpc_a & >Hr1 & >Hr2) Hϕ".
@@ -328,17 +327,17 @@ Section cap_lang_rules.
      iDestruct (@gen_heap_valid with "Hr HPC") as %?.
      iDestruct (@gen_heap_valid with "Hr Hr2") as %?.
      option_locate_mr m r.
-     assert (<[PC:=inr (pc_p, pc_g, a1, if (a2 =? -42)%a then None
-                                   else Some a2, pc_a)]>
-             r !r! PC = inr (pc_p, pc_g, a1, if (a2 =? -42)%a then None
-                                   else Some a2, pc_a))
+     assert (<[PC:=inr (pc_p, pc_g, a1, if (a2 =? -42)%a then (A MemNum eq_refl)
+                                   else a2, pc_a)]>
+             r !r! PC = inr (pc_p, pc_g, a1, if (a2 =? -42)%a then (A MemNum eq_refl)
+                                   else a2, pc_a))
        as Hpc_new1; first by rewrite /RegLocate lookup_insert.
      iApply fupd_frame_l.
      iSplit.
      - rewrite /reducible.
        iExists [], (Instr _),
        (updatePC (update_reg (r,m) PC (inr ((pc_p, pc_g), a1,
-            if (a2 =? (-42))%a then None else Some a2, pc_a)))).2,[].
+            if (a2 =? (-42))%a then (A MemNum eq_refl) else a2, pc_a)))).2,[].
        iPureIntro.
        constructor.
        apply (step_exec_instr (r,m) pc_p pc_g pc_b pc_e pc_a
@@ -506,102 +505,98 @@ Section cap_lang_rules.
          iSpecialize ("Hϕ" with "[HPC Ha]"); iFrame; eauto ).
    Qed.
 
- (* (* --------------------------------------------------------------------------------- *) *)
- (* (* ----------------------------------- FAIL RULES ---------------------------------- *) *)
+ (* --------------------------------------------------------------------------------- *)
+ (* ----------------------------------- FAIL RULES ---------------------------------- *)
 
- (*  Lemma wp_notCorrectPC: *)
- (*    forall pc_p pc_g pc_b pc_e pc_a, *)
- (*      ~ isCorrectPC (inr ((pc_p,pc_g),pc_b,pc_e,pc_a)) -> *)
- (*      {{{ PC ↦ᵣ inr ((pc_p,pc_g),pc_b,pc_e,pc_a) }}} *)
- (*        Executable *)
- (*        {{{ RET FailedV; True }}}. *)
- (*  Proof. *)
- (*    intros until 0. intros Hnpc. *)
- (*    iIntros (ϕ) "HPC Hϕ". *)
- (*    iApply wp_lift_step_fupd; eauto. *)
- (*    iIntros (σ1 l1 l2 n) "Hσ1 /="; destruct σ1; simpl; *)
- (*    iDestruct "Hσ1" as "[Hr Hm]". *)
- (*    iDestruct (@gen_heap_valid with "Hr HPC") as %?. *)
- (*    option_locate_mr m r. *)
- (*    rewrite -HPC in Hnpc. *)
- (*    iApply fupd_frame_l.  *)
- (*    iSplit. *)
- (*    + rewrite /reducible. *)
- (*      iExists [], (Failed : cap_lang.expr), (r,m), []. *)
- (*      iPureIntro. *)
- (*      constructor. *)
- (*      apply (step_exec_fail (r,m)); eauto. *)
- (*    + iMod (fupd_intro_mask' ⊤) as "H"; eauto. *)
- (*      iModIntro.  *)
- (*      iIntros (e1 σ2 efs Hstep). *)
- (*      inv_head_step_advanced m r HPC Hpc_a Hinstr Hstep HPC. *)
- (*      iFrame. iModIntro. iNext. *)
- (*      iApply fupd_frame_l. iFrame. *)
- (*      iApply wp_value. iApply "Hϕ". *)
- (*      auto. *)
- (*  Qed. *)
+  Lemma wp_notCorrectPC:
+    forall E pc_p pc_g pc_b pc_e pc_a,
+      ~ isCorrectPC (inr ((pc_p,pc_g),pc_b,pc_e,pc_a)) ->
+      {{{ PC ↦ᵣ inr ((pc_p,pc_g),pc_b,pc_e,pc_a) }}}
+        Instr Executable @ E
+        {{{ RET FailedV; True }}}.
+  Proof.
+    intros until 0. intros Hnpc.
+    iIntros (ϕ) "HPC Hϕ".
+    iApply wp_lift_atomic_head_step_no_fork; auto.
+    iIntros (σ1 l1 l2 n) "Hσ1 /="; destruct σ1; simpl;
+    iDestruct "Hσ1" as "[Hr Hm]".
+    iDestruct (@gen_heap_valid with "Hr HPC") as %?.
+    option_locate_mr m r.
+    rewrite -HPC in Hnpc.
+    iApply fupd_frame_l.
+    iSplit.
+    + rewrite /reducible.
+      iExists [], (Instr Failed : cap_lang.expr), (r,m), [].
+      iPureIntro.
+      constructor. 
+      apply (step_exec_fail (r,m)); eauto.
+    + (* iMod (fupd_intro_mask' ⊤) as "H"; eauto. *)
+      iModIntro.
+      iIntros (e1 σ2 efs Hstep).
+      inv_head_step_advanced m r HPC Hpc_a Hinstr Hstep HPC.
+      iFrame. iNext.
+      iModIntro. iSplitR; auto. by iApply "Hϕ".
+  Qed.
   
- (*   Lemma wp_load_fail1 r1 r2 pc_p pc_g pc_b pc_e pc_a w p g b e a : *)
- (*    cap_lang.decode w = Load r1 r2 → *)
+   Lemma wp_load_fail1 E r1 r2 pc_p pc_g pc_b pc_e pc_a w p g b e a :
+    cap_lang.decode w = Load r1 r2 →
 
- (*    isCorrectPC (inr ((pc_p,pc_g),pc_b,pc_e,pc_a)) ∧ *)
- (*     (readAllowed p = false ∨ withinBounds ((p, g), b, e, a) = false) → *)
+    isCorrectPC (inr ((pc_p,pc_g),pc_b,pc_e,pc_a)) ∧
+     (readAllowed p = false ∨ withinBounds ((p, g), b, e, a) = false) →
 
- (*    {{{ PC ↦ᵣ inr ((pc_p,pc_g),pc_b,pc_e,pc_a) *)
- (*           ∗ pc_a ↦ₐ w *)
- (*           ∗ r2 ↦ᵣ inr ((p,g),b,e,a) }}} *)
- (*      Executable *)
- (*    {{{ RET FailedV; True }}}. *)
- (*   Proof. *)
- (*     intros Hinstr [Hvpc [Hnra | Hnwb]]; *)
- (*     (iIntros (φ) "(HPC & Hpc_a & Hr2) Hφ"; *)
- (*       iApply wp_lift_step_fupd; eauto; *)
- (*       iIntros (σ1 l1 l2 n) "Hσ1 /="; destruct σ1; simpl; *)
- (*       iDestruct "Hσ1" as "[Hr Hm]"; *)
- (*       iDestruct (@gen_heap_valid with "Hr HPC") as %?; *)
- (*       iDestruct (@gen_heap_valid with "Hm Hpc_a") as %?; *)
- (*       iDestruct (@gen_heap_valid with "Hr Hr2") as %?; *)
- (*       option_locate_mr m r). *)
- (*     - iApply fupd_frame_l.  *)
- (*       iSplit. *)
- (*       + rewrite /reducible. *)
- (*         iExists [], Failed, (r,m), []. *)
- (*         iPureIntro. *)
- (*         constructor. *)
- (*         apply (step_exec_instr (r,m) pc_p pc_g pc_b pc_e pc_a (Load r1 r2) *)
- (*                                (Failed,_)); *)
- (*           eauto; simpl; try congruence.  *)
- (*           by rewrite Hr2 Hnra /=. *)
- (*       + iMod (fupd_intro_mask' ⊤) as "H"; eauto. *)
- (*         iModIntro.  *)
- (*         iIntros (e1 σ2 efs Hstep). *)
- (*         inv_head_step_advanced m r HPC Hpc_a Hinstr Hstep HPC. *)
- (*         rewrite Hr2 Hnra /=. *)
- (*         iFrame. iModIntro. iNext. *)
- (*         iApply fupd_frame_l. iFrame. *)
- (*         iApply wp_value. by iApply "Hφ". *)
- (*     - simpl in *.  *)
- (*       iApply fupd_frame_l.  *)
- (*       iSplit. *)
- (*       + rewrite /reducible. *)
- (*         iExists [], Failed, (r,m), []. *)
- (*         iPureIntro. *)
- (*         constructor. *)
- (*         apply (step_exec_instr (r,m) pc_p pc_g pc_b pc_e pc_a (Load r1 r2) *)
- (*                                (Failed,_)); *)
- (*           eauto; simpl; try congruence. *)
- (*           by rewrite Hr2 Hnwb andb_false_r.  *)
- (*       + iMod (fupd_intro_mask' ⊤) as "H"; eauto. *)
- (*         iModIntro.  *)
- (*         iIntros (e1 σ2 efs Hstep). *)
- (*         inv_head_step_advanced m r HPC Hpc_a Hinstr Hstep HPC. *)
- (*         rewrite Hr2 Hnwb andb_false_r.  *)
- (*         iFrame. iModIntro. iNext. *)
- (*         iApply fupd_frame_l. iFrame. *)
- (*         iApply wp_value. by iApply "Hφ". *)
- (*   Qed. *)
+    {{{ PC ↦ᵣ inr ((pc_p,pc_g),pc_b,pc_e,pc_a)
+           ∗ pc_a ↦ₐ w
+           ∗ r2 ↦ᵣ inr ((p,g),b,e,a) }}}
+      Instr Executable @ E
+    {{{ RET FailedV; True }}}.
+   Proof.
+     intros Hinstr [Hvpc [Hnra | Hnwb]];
+     (iIntros (φ) "(HPC & Hpc_a & Hr2) Hφ";
+       iApply wp_lift_atomic_head_step_no_fork; auto;
+       iIntros (σ1 l1 l2 n) "Hσ1 /="; destruct σ1; simpl;
+       iDestruct "Hσ1" as "[Hr Hm]";
+       iDestruct (@gen_heap_valid with "Hr HPC") as %?;
+       iDestruct (@gen_heap_valid with "Hm Hpc_a") as %?;
+       iDestruct (@gen_heap_valid with "Hr Hr2") as %?;
+       option_locate_mr m r).
+     - iApply fupd_frame_l.
+       iSplit.
+       + rewrite /reducible.
+         iExists [], (Instr Failed), (r,m), [].
+         iPureIntro.
+         constructor.
+         apply (step_exec_instr (r,m) pc_p pc_g pc_b pc_e pc_a (Load r1 r2)
+                                (Failed,_));
+           eauto; simpl; try congruence.
+           by rewrite Hr2 Hnra /=.
+       + (* iMod (fupd_intro_mask' ⊤) as "H"; eauto. *)
+         iModIntro.
+         iIntros (e1 σ2 efs Hstep).
+         inv_head_step_advanced m r HPC Hpc_a Hinstr Hstep HPC.
+         rewrite Hr2 Hnra /=.
+         iFrame. iNext. iModIntro.
+         iSplitR; auto. by iApply "Hφ".
+     - simpl in *.
+       iApply fupd_frame_l.
+       iSplit.
+       + rewrite /reducible.
+         iExists [], (Instr Failed), (r,m), [].
+         iPureIntro.
+         constructor.
+         apply (step_exec_instr (r,m) pc_p pc_g pc_b pc_e pc_a (Load r1 r2)
+                                (Failed,_));
+           eauto; simpl; try congruence.
+           by rewrite Hr2 Hnwb andb_false_r.
+       + (* iMod (fupd_intro_mask' ⊤) as "H"; eauto. *)
+         iModIntro.
+         iIntros (e1 σ2 efs Hstep).
+         inv_head_step_advanced m r HPC Hpc_a Hinstr Hstep HPC.
+         rewrite Hr2 Hnwb andb_false_r.
+         iFrame. iNext.
+         iSplitR; auto. by iApply "Hφ".
+   Qed.
 
- (*   Lemma wp_load_fail2 r1 r2 pc_p pc_g pc_b pc_e pc_a w n: *)
+   (* Lemma wp_load_fail2 r1 r2 pc_p pc_g pc_b pc_e pc_a w n: *)
  (*    cap_lang.decode w = Load r1 r2 → *)
 
  (*    isCorrectPC (inr ((pc_p,pc_g),pc_b,pc_e,pc_a)) → *)
@@ -631,7 +626,7 @@ Section cap_lang_rules.
  (*         eauto; simpl; try congruence. *)
  (*         by rewrite Hr2. *)
  (*     - iMod (fupd_intro_mask' ⊤) as "H"; eauto. *)
- (*       iModIntro.  *)
+ (*       iModIntro. *)
  (*       iIntros (e1 σ2 efs Hstep). *)
  (*       inv_head_step_advanced m r HPC Hpc_a Hinstr Hstep HPC. *)
  (*       rewrite Hr2 /=. *)
@@ -661,7 +656,7 @@ Section cap_lang_rules.
  (*      iDestruct (@gen_heap_valid with "Hm Hpc_a") as %?; *)
  (*      iDestruct (@gen_heap_valid with "Hr Hdst") as %?; *)
  (*      option_locate_mr m r). *)
- (*     iApply fupd_frame_l.  *)
+ (*     iApply fupd_frame_l. *)
  (*     iSplit. *)
  (*     - rewrite /reducible. *)
  (*       iExists [], Failed, (r,m), []. *)
@@ -677,16 +672,16 @@ Section cap_lang_rules.
  (*         rewrite andb_comm; simpl; auto. *)
  (*         destruct src; auto. *)
  (*     - iMod (fupd_intro_mask' ⊤) as "H"; eauto. *)
- (*       iModIntro.  *)
+ (*       iModIntro. *)
  (*       iIntros (e1 σ2 efs Hstep). *)
  (*       inv_head_step_advanced m r HPC Hpc_a Hinstr Hstep HPC. *)
  (*       rewrite Hdst. destruct HnwaHnwb as [Hnwa | Hnwb]. *)
  (*       + rewrite Hnwa; simpl. destruct src; simpl. *)
  (*         * iFrame. iModIntro. iNext. *)
- (*           iApply fupd_frame_l. iFrame.          *)
+ (*           iApply fupd_frame_l. iFrame. *)
  (*           iApply wp_value. by iApply "Hφ". *)
  (*         * iFrame. iModIntro. iNext. *)
- (*           iApply fupd_frame_l. iFrame.          *)
+ (*           iApply fupd_frame_l. iFrame. *)
  (*           iApply wp_value. by iApply "Hφ". *)
  (*       + simpl in Hnwb. rewrite Hnwb. *)
  (*         rewrite andb_comm; simpl. *)
@@ -729,7 +724,7 @@ Section cap_lang_rules.
  (*         eauto; simpl; try congruence. *)
  (*         destruct src; simpl; by rewrite Hdst. *)
  (*     - iMod (fupd_intro_mask' ⊤) as "H"; eauto. *)
- (*       iModIntro.  *)
+ (*       iModIntro. *)
  (*       iIntros (e1 σ2 efs Hstep). *)
  (*       inv_head_step_advanced m r HPC Hpc_a Hinstr Hstep HPC. *)
  (*       rewrite Hdst /=. *)
@@ -782,7 +777,7 @@ Section cap_lang_rules.
  (*       rewrite Hsrc. rewrite Hloc. *)
  (*       destruct p; try congruence. *)
  (*     - iMod (fupd_intro_mask' ⊤) as "H"; eauto. *)
- (*       iModIntro.  *)
+ (*       iModIntro. *)
  (*       iIntros (e1 σ2 efs Hstep). *)
  (*       inv_head_step_advanced m r HPC Hpc_a Hinstr Hstep HPC. *)
  (*       rewrite Hdst. rewrite Hwa. simpl in Hwb. rewrite Hwb. simpl. *)
@@ -833,7 +828,7 @@ Section cap_lang_rules.
  (*       + destruct HpHa as [Hp | Ha]; try congruence. *)
  (*         rewrite Ha. destruct p; auto. *)
  (*     - iMod (fupd_intro_mask' ⊤) as "H"; eauto. *)
- (*       iModIntro.  *)
+ (*       iModIntro. *)
  (*       iIntros (e1 σ2 efs Hstep). *)
  (*       inv_head_step_advanced m r HPC Hpc_a Hinstr Hstep HPC. *)
  (*       rewrite Hdst. assert (X:match p with *)
@@ -851,7 +846,7 @@ Section cap_lang_rules.
  (*           rewrite Ha. destruct p; auto. } *)
  (*       repeat rewrite X. *)
  (*       iFrame. iModIntro. iNext. *)
- (*       iApply fupd_frame_l. iFrame.          *)
+ (*       iApply fupd_frame_l. iFrame. *)
  (*       iApply wp_value. by iApply "Hφ". *)
  (*   Qed. *)
 
@@ -885,7 +880,7 @@ Section cap_lang_rules.
  (*         eauto; simpl; try congruence. *)
  (*         destruct src; simpl; by rewrite Hdst. *)
  (*     - iMod (fupd_intro_mask' ⊤) as "H"; eauto. *)
- (*       iModIntro.  *)
+ (*       iModIntro. *)
  (*       iIntros (e1 σ2 efs Hstep). *)
  (*       inv_head_step_advanced m r HPC Hpc_a Hinstr Hstep HPC. *)
  (*       rewrite Hdst /=. *)
@@ -930,12 +925,12 @@ Section cap_lang_rules.
  (*         eauto; simpl; try congruence. *)
  (*       rewrite Hdst. subst p; auto. *)
  (*     - iMod (fupd_intro_mask' ⊤) as "H"; eauto. *)
- (*       iModIntro.  *)
+ (*       iModIntro. *)
  (*       iIntros (e1 σ2 efs Hstep). *)
  (*       inv_head_step_advanced m r HPC Hpc_a Hinstr Hstep HPC. *)
  (*       rewrite Hdst. subst p. *)
  (*       iFrame. iModIntro. iNext. *)
- (*       iApply fupd_frame_l. iFrame.          *)
+ (*       iApply fupd_frame_l. iFrame. *)
  (*       iApply wp_value. by iApply "Hφ". *)
  (*   Qed. *)
    
@@ -975,14 +970,14 @@ Section cap_lang_rules.
  (*       rewrite Hdst. rewrite Hrg. rewrite Ha. *)
  (*       destruct p; auto. *)
  (*     - iMod (fupd_intro_mask' ⊤) as "H"; eauto. *)
- (*       iModIntro.  *)
+ (*       iModIntro. *)
  (*       iIntros (e1 σ2 efs Hstep). *)
  (*       inv_head_step_advanced m r HPC Hpc_a Hinstr Hstep HPC. *)
  (*       rewrite Hdst. rewrite Hrg. rewrite Ha. *)
  (*       assert (X: match p with | O | _ => (Failed, (r, m)) end = (Failed, (r, m))) by (destruct p; auto). *)
  (*       rewrite X. *)
  (*       iFrame. iModIntro. iNext. *)
- (*       iApply fupd_frame_l. iFrame.          *)
+ (*       iApply fupd_frame_l. iFrame. *)
  (*       iApply wp_value. by iApply "Hφ". *)
  (*   Qed. *)
 
@@ -1021,14 +1016,14 @@ Section cap_lang_rules.
  (*       rewrite Hdst. rewrite Hrg. *)
  (*       destruct p; auto. *)
  (*     - iMod (fupd_intro_mask' ⊤) as "H"; eauto. *)
- (*       iModIntro.  *)
+ (*       iModIntro. *)
  (*       iIntros (e1 σ2 efs Hstep). *)
  (*       inv_head_step_advanced m r HPC Hpc_a Hinstr Hstep HPC. *)
  (*       rewrite Hdst. rewrite Hrg. *)
  (*       assert (X: match p with | O | _ => (Failed, (r, m)) end = (Failed, (r, m))) by (destruct p; auto). *)
  (*       rewrite X. *)
  (*       iFrame. iModIntro. iNext. *)
- (*       iApply fupd_frame_l. iFrame.          *)
+ (*       iApply fupd_frame_l. iFrame. *)
  (*       iApply wp_value. by iApply "Hφ". *)
  (*   Qed. *)
 
@@ -1063,14 +1058,14 @@ Section cap_lang_rules.
  (*         eauto; simpl; try congruence. *)
  (*       rewrite Hdst. destruct src; auto. *)
  (*     - iMod (fupd_intro_mask' ⊤) as "H"; eauto. *)
- (*       iModIntro.  *)
+ (*       iModIntro. *)
  (*       iIntros (e1 σ2 efs Hstep). *)
  (*       inv_head_step_advanced m r HPC Hpc_a Hinstr Hstep HPC. *)
- (*       rewrite Hdst.  *)
+ (*       rewrite Hdst. *)
  (*       assert (X: match src with | inl _ | _ => (Failed, (r, m)) end = (Failed, (r, m))) by (destruct src; auto). *)
  (*       rewrite X. *)
  (*       iFrame. iModIntro. iNext. *)
- (*       iApply fupd_frame_l. iFrame.          *)
+ (*       iApply fupd_frame_l. iFrame. *)
  (*       iApply wp_value. by iApply "Hφ". *)
  (*   Qed. *)
 
@@ -1107,12 +1102,12 @@ Section cap_lang_rules.
  (*         eauto; simpl; try congruence. *)
  (*       rewrite Hdst. rewrite Hsrc. auto. *)
  (*     - iMod (fupd_intro_mask' ⊤) as "H"; eauto. *)
- (*       iModIntro.  *)
+ (*       iModIntro. *)
  (*       iIntros (e1 σ2 efs Hstep). *)
  (*       inv_head_step_advanced m r HPC Hpc_a Hinstr Hstep HPC. *)
  (*       rewrite Hdst. rewrite Hsrc. *)
  (*       iFrame. iModIntro. iNext. *)
- (*       iApply fupd_frame_l. iFrame.          *)
+ (*       iApply fupd_frame_l. iFrame. *)
  (*       iApply wp_value. by iApply "Hφ". *)
  (*   Qed. *)
 
@@ -1156,23 +1151,23 @@ Section cap_lang_rules.
  (*         eauto; simpl; try congruence. *)
  (*         rewrite Hr1. destruct y; auto. *)
  (*     - iMod (fupd_intro_mask' ⊤) as "H"; eauto. *)
- (*       iModIntro.  *)
+ (*       iModIntro. *)
  (*       iIntros (e1 σ2 efs Hstep). destruct Hinstr as [Hinstr | [Hinstr | Hinstr]]; *)
  (*       inv_head_step_advanced m r HPC Hpc_a Hinstr Hstep HPC. *)
  (*       + rewrite Hr1. assert (X: match y with | inl _ | _ => (Failed, (r, m)) end = (Failed, (r, m))) by (destruct y; auto). *)
  (*         rewrite X. *)
  (*         iFrame. iModIntro. iNext. *)
- (*         iApply fupd_frame_l. iFrame.          *)
+ (*         iApply fupd_frame_l. iFrame. *)
  (*         iApply wp_value; by iApply "Hφ". *)
  (*       + rewrite Hr1. assert (X: match y with | inl _ | _ => (Failed, (r, m)) end = (Failed, (r, m))) by (destruct y; auto). *)
  (*         rewrite X. *)
  (*         iFrame. iModIntro. iNext. *)
- (*         iApply fupd_frame_l. iFrame.          *)
+ (*         iApply fupd_frame_l. iFrame. *)
  (*         iApply wp_value; by iApply "Hφ". *)
  (*       + rewrite Hr1. assert (X: match y with | inl _ | _ => (Failed, (r, m)) end = (Failed, (r, m))) by (destruct y; auto). *)
  (*         rewrite X. *)
  (*         iFrame. iModIntro. iNext. *)
- (*         iApply fupd_frame_l. iFrame.          *)
+ (*         iApply fupd_frame_l. iFrame. *)
  (*         iApply wp_value; by iApply "Hφ". *)
  (*   Qed. *)
 
@@ -1216,7 +1211,7 @@ Section cap_lang_rules.
  (*         eauto; simpl; try congruence. *)
  (*         rewrite Hr2. destruct x; auto. destruct (r !r! r0); auto. *)
  (*     - iMod (fupd_intro_mask' ⊤) as "H"; eauto. *)
- (*       iModIntro.  *)
+ (*       iModIntro. *)
  (*       iIntros (e1 σ2 efs Hstep). destruct Hinstr as [Hinstr | [Hinstr | Hinstr]]; *)
  (*       inv_head_step_advanced m r HPC Hpc_a Hinstr Hstep HPC. *)
  (*       + rewrite Hr2. assert (X: match x with *)
@@ -1228,7 +1223,7 @@ Section cap_lang_rules.
  (*         { destruct x; auto. destruct (r !r! r0); auto. } *)
  (*         rewrite X. *)
  (*         iFrame. iModIntro. iNext. *)
- (*         iApply fupd_frame_l. iFrame.          *)
+ (*         iApply fupd_frame_l. iFrame. *)
  (*         iApply wp_value; by iApply "Hφ". *)
  (*       + rewrite Hr2. assert (X: match x with *)
  (*                  | inl _ => (Failed, (r, m)) *)
@@ -1239,7 +1234,7 @@ Section cap_lang_rules.
  (*         { destruct x; auto. destruct (r !r! r0); auto. } *)
  (*         rewrite X. *)
  (*         iFrame. iModIntro. iNext. *)
- (*         iApply fupd_frame_l. iFrame.          *)
+ (*         iApply fupd_frame_l. iFrame. *)
  (*         iApply wp_value; by iApply "Hφ". *)
  (*       + rewrite Hr2. assert (X: match x with *)
  (*                  | inl _ => (Failed, (r, m)) *)
@@ -1250,7 +1245,7 @@ Section cap_lang_rules.
  (*         { destruct x; auto. destruct (r !r! r0); auto. } *)
  (*         rewrite X. *)
  (*         iFrame. iModIntro. iNext. *)
- (*         iApply fupd_frame_l. iFrame.          *)
+ (*         iApply fupd_frame_l. iFrame. *)
  (*         iApply wp_value; by iApply "Hφ". *)
  (*   Qed. *)
 
@@ -1264,21 +1259,21 @@ Section cap_lang_rules.
  (*     isCorrectPC (inr ((pc_p,pc_g),pc_b,pc_e,pc_a)) → *)
      
  (*     {{{ PC ↦ᵣ inr ((pc_p,pc_g),pc_b,pc_e,pc_a) ∗ pc_a ↦ₐ w }}} *)
- (*       Executable  *)
+ (*       Executable *)
  (*     {{{ RET HaltedV; PC ↦ᵣ inr ((pc_p,pc_g),pc_b,pc_e,pc_a) ∗ pc_a ↦ₐ w }}}. *)
  (*   Proof. *)
- (*     intros Hinstr Hvpc.  *)
+ (*     intros Hinstr Hvpc. *)
  (*     iIntros (φ) "[Hpc Hpca] Hφ". *)
  (*     iApply wp_lift_atomic_step_fupd; auto. *)
  (*     iIntros (σ1 l1 l2 n) "Hσ1 /=". destruct σ1; simpl. *)
  (*     iDestruct "Hσ1" as "[Hr Hm]". *)
  (*     iDestruct (@gen_heap_valid with "Hr Hpc") as %?. *)
  (*     iDestruct (@gen_heap_valid with "Hm Hpca") as %?. *)
- (*     option_locate_mr m r.  *)
+ (*     option_locate_mr m r. *)
  (*     iModIntro. *)
  (*     iSplitR. *)
- (*     - rewrite /reducible.  *)
- (*       iExists [],Halted,(r,m),[].        *)
+ (*     - rewrite /reducible. *)
+ (*       iExists [],Halted,(r,m),[]. *)
  (*       iPureIntro. *)
  (*       constructor. *)
  (*       apply (step_exec_instr (r,m) pc_p pc_g pc_b pc_e pc_a Halt *)
@@ -1287,7 +1282,7 @@ Section cap_lang_rules.
  (*     - iIntros (e2 σ2 efs Hstep). *)
  (*       inv_head_step_advanced m r HPC Hpc_a Hinstr Hstep HPC. *)
  (*       iFrame. *)
- (*       iModIntro. iNext. iModIntro. iSplitL; eauto.  *)
+ (*       iModIntro. iNext. iModIntro. iSplitL; eauto. *)
  (*       iApply "Hφ". *)
  (*       iFrame. *)
  (*   Qed. *)
@@ -1297,21 +1292,21 @@ Section cap_lang_rules.
  (*     isCorrectPC (inr ((pc_p,pc_g),pc_b,pc_e,pc_a)) → *)
      
  (*     {{{ PC ↦ᵣ inr ((pc_p,pc_g),pc_b,pc_e,pc_a) ∗ pc_a ↦ₐ w }}} *)
- (*       Executable  *)
+ (*       Executable *)
  (*     {{{ RET FailedV; PC ↦ᵣ inr ((pc_p,pc_g),pc_b,pc_e,pc_a) ∗ pc_a ↦ₐ w }}}. *)
  (*   Proof. *)
- (*     intros Hinstr Hvpc.  *)
+ (*     intros Hinstr Hvpc. *)
  (*     iIntros (φ) "[Hpc Hpca] Hφ". *)
  (*     iApply wp_lift_atomic_step_fupd; auto. *)
  (*     iIntros (σ1 l1 l2 n) "Hσ1 /=". destruct σ1; simpl. *)
  (*     iDestruct "Hσ1" as "[Hr Hm]". *)
  (*     iDestruct (@gen_heap_valid with "Hr Hpc") as %?. *)
  (*     iDestruct (@gen_heap_valid with "Hm Hpca") as %?. *)
- (*     option_locate_mr m r.  *)
+ (*     option_locate_mr m r. *)
  (*     iModIntro. *)
  (*     iSplitR. *)
- (*     - rewrite /reducible.  *)
- (*       iExists [],Failed,(r,m),[].        *)
+ (*     - rewrite /reducible. *)
+ (*       iExists [],Failed,(r,m),[]. *)
  (*       iPureIntro. *)
  (*       constructor. *)
  (*       apply (step_exec_instr (r,m) pc_p pc_g pc_b pc_e pc_a Fail *)
@@ -1320,10 +1315,10 @@ Section cap_lang_rules.
  (*     - iIntros (e2 σ2 efs Hstep). *)
  (*       inv_head_step_advanced m r HPC Hpc_a Hinstr Hstep HPC. *)
  (*       iFrame. *)
- (*       iModIntro. iNext. iModIntro. iSplitL; eauto.  *)
+ (*       iModIntro. iNext. iModIntro. iSplitL; eauto. *)
  (*       iApply "Hφ". *)
  (*       iFrame. *)
-  (*   Qed. *)
+ (*    Qed. *)
 
 
  (* --------------------------------------------------------------------------------- *)
